LeanProjeto2/StarLanguage/FiniteTypes.lean
@@ -1,0 +1,46 @@
+-- -------------------------------------------------------------
+--            STAR LANGUAGE - FINITE TYPES
+-- -------------------------------------------------------------
+
+-- We import the definitions from the first-order language L:
+import LeanProjeto2.FOLanguage
+import MathLib.Tactic                   -- Pergunta: é preciso repetir isto?
+
+open FOLang
+open LFormula
+
+-- ----------------------
+-- FINITE TYPES
+-- ----------------------
+
+-- Finite types [def 1.1]
+inductive FType : Type
+| ground : FType                        -- G
+| arrow : FType → FType → FType         -- σ → τ
+| star : FType → FType                  -- σ*
+deriving Repr, DecidableEq
+
+open FType
+
+-- Notation for finite types
+def G := ground                         -- notation G => ground
+notation t "⟶" t1 => arrow t t1
+notation t "⋆" => star t
+
+-- EXAMPLE:
+def s1ex2_1 : FType := G⋆
+def s1ex2_2 : FType := G ⟶ G
+def s1ex2_3 : FType := G ⟶ (G ⟶ G)
+def s1ex2_3' : FType := (G ⟶ G) ⟶ G
+def s1ex2_4 : FType := (G ⟶ G) ⟶ (G ⟶ (G ⟶ G))
+def s1ex2_5 (σ τ : FType) : FType := σ ⟶ ((σ⋆ ⟶ τ) ⟶ τ)
+def s1ex2_5' (σ τ : FType) : FType := (σ⋆ ⟶ τ)⋆
+example (σ τ : FType) : FType := (σ⋆ ⟶ τ)⋆
+
+-- DEFINITION (Tuple of Types): We define tuples of types as lists
+def FTypeTuple := List FType
+deriving Repr, DecidableEq
+
+-- EXAMPLE: two examples of tuples
+def exTuple1 : FTypeTuple := [G]
+def exTuple2 : FTypeTuple := [G⋆,G ⟶ G]
