LeanProjeto2/StarLanguage/ResultsAndOtherDefinitions.lean
@@ -1,0 +1,13 @@
+-- -------------------------------------------------------------
+--       STAR LANGUAGE - RESULTS and OTHER DEFINITIONS
+-- -------------------------------------------------------------
+
+-- We import the definitions from the first-order language L:
+import LeanProjeto2.FOLanguage
+import LeanProjeto2.StarLanguage.FiniteTypes
+import LeanProjeto2.StarLanguage.Syntax
+import LeanProjeto2.StarLanguage.Axioms
+import MathLib.Tactic
+
+open FOLang
+open LFormula
