LeanProjeto2/StarLanguage/Syntax.lean
@@ -1,0 +1,606 @@
+-- -------------------------------------------------------------
+--            STAR LANGUAGE - THE SYNTAX
+-- -------------------------------------------------------------
+
+-- We import the definitions from the first-order language L:
+import LeanProjeto2.FOLanguage
+import LeanProjeto2.StarLanguage.FiniteTypes
+import MathLib.Tactic
+import Init.Data.List.Basic
+import Init.Data.List.Lemmas
+
+open FOLang
+open LFormula
+
+-- ----------------------------
+-- TERMS and CONSTANTS (p.9-12)
+-- ----------------------------
+
+-- DEFINITION 1.2 (p.8-9): Terms of L^{omega}_*
+inductive Term --where
+| lcons : LTerm → Term                  -- L-constants
+| pi --{σ τ: FType} : Term                                    -- combinators:     Π
+| sigma --{σ τ ρ: FType} : Term                               --                  Σ
+| sing                                  -- star constants:  𝔰
+| bUnion                                --                  ∪ (binary union)
+| iUnion                                --                  ∪ (indexed union)
+| var : String → Term                   -- variables
+| app : Term → Term → Term              -- application of terms
+deriving Repr, DecidableEq
+
+open Term
+
+-- EXAMPLE: some terms to use in future examples
+def var_x := var "x"
+def var_y := var "y"
+def var_z := var "z"
+def lcons_a (a:LTerm) := lcons a
+def lcons_k (k:LTerm) := lcons k
+def lcons_var_y := lcons (Lvar_y)
+
+-- --------------------------------
+-- TERMS OF TUPLES (new)
+-- --------------------------------
+
+def TermTuple := List Term
+deriving BEq, Repr
+
+-- This function takes a list of Term and makes a term tuple out of it
+def makeTuple (ts : List Term) : TermTuple := ts
+
+-- We define a function in order to access any element in the tuple
+def getElement (n : Nat) (t : TermTuple) : Option Term :=           -- Option para ter some/none para o caso do tuple ter 2 elementos e pedirmos o terceiro
+  List.get? t n
+
+-- -------
+-- EXAMPLE: a tuple of terms + access to its elements (new)
+-- -------
+
+def exTermTuple : TermTuple := makeTuple ([var_x, var_y])  -- a tuple of terms (a list with the terms x and a)
+
+#eval getElement 0 exTermTuple          -- Output: var_x (the first element of exTermTuple)
+#eval getElement 1 exTermTuple          -- Output: var_y (the second element of exTermTuple)
+#eval getElement 2 exTermTuple          -- Output: none (there is no third element in exTermTuple)
+
+
+-- --------------------------------
+-- WELL-FORMED TERMS
+-- --------------------------------
+
+-- Helper function to check if an LTerm is well-formed        TODO: Repetido no FOLanguage as LTerm_is_wellformed
+inductive LTerm_is_wellformed_inStar : List String → LTerm → Prop
+-- a variable is well-formed if that variable is in the given list of variables
+| wf_var {xs x} : x ∈ xs → LTerm_is_wellformed_inStar xs (LTerm.Lvar x)
+| wf_const {xs c} : LTerm_is_wellformed_inStar xs (LTerm.Lconst c)
+| wf_func {xs f ts} : (∀ t ∈ ts, LTerm_is_wellformed_inStar xs t) → LTerm_is_wellformed_inStar xs (LTerm.Lfunc f ts)
+
+-- Define Term_is_wellformed for Term
+inductive Term_is_wellformed : List String → Term → Prop
+| wf_lcons {xs} {t : LTerm} : LTerm_is_wellformed_inStar xs t → Term_is_wellformed xs (lcons t)           -- TODO not now: não sei porque com LTerm.LTerm_is_wellformed não funciona tbm
+| wf_pi {xs} : Term_is_wellformed xs pi
+| wf_sigma {xs} : Term_is_wellformed xs sigma
+| wf_sing {xs} : Term_is_wellformed xs sing
+| wf_bUnion {xs} : Term_is_wellformed xs bUnion
+| wf_iUnion {xs} : Term_is_wellformed xs iUnion
+| wf_var {xs x} : x ∈ xs → Term_is_wellformed xs (var x)
+| wf_app {xs t1 t2} : Term_is_wellformed xs t1 → Term_is_wellformed xs t2 → Term_is_wellformed xs (app t1 t2)
+
+-- Definition: well-formed tuple of terms (new)
+inductive TermTuple_is_wellformed : List String → List Term → Prop
+| wf_tuple : (∀ t ∈ ts, Term_is_wellformed xs t) → (TermTuple_is_wellformed xs ts)
+
+-- --------
+-- Example:
+-- --------
+
+-- Next example: mostrar que var_x is well-formed under the list of variables ["x", "y"]
+-- (List.mem_cons_self "x" ["y"]) states que "x" pertence à lista [ "x","y" ]
+example : Term_is_wellformed ["x", "y"] var_x := Term_is_wellformed.wf_var (List.mem_cons_self "x" ["y"])
+
+-- --------------------------------
+-- SUBTERM
+-- --------------------------------
+
+namespace Term
+
+-- DEFINITION: subterm of a term
+inductive isSubterm : Term → Term → Prop
+| refl (t : Term) : isSubterm t t                                                             -- Terms are always subterms of themselves
+| app_left {t₁ t₂ t' : Term} : isSubterm t' t₁ → isSubterm t' (Term.app t₁ t₂)                  -- Subterms of applications (LHS)
+| app_right {t₁ t₂ t' : Term} : isSubterm t' t₂ → isSubterm t' (Term.app t₁ t₂)                 -- Subterms of applications (RHS)
+
+open isSubterm
+
+-- Example: example of a subterm
+example : isSubterm (var "x") (app (var "x") (var "y")) :=
+  by
+    have H := isSubterm.refl (var "x")
+    exact app_left H
+
+/-
+-- Examples of subterms
+example : isSubterm (var "x") ((var "x")·(var "y")) :=
+  app_left refl
+
+example : isSubterm (Term.var "y") (Term.app (Term.var "x") (Term.var "y")) :=
+  app_right refl
+-/
+
+-- DEFINITION: subterm of a tuple of terms
+inductive isSubtermTuple : TermTuple → TermTuple → Prop
+| empty_subtuple : isSubtermTuple [] []                                      -- Empty tuple is a subtuple of itself
+| rec_subtuple {t₁ t₂ : Term} {ts₁ ts₂ : TermTuple} :                       -- Recursive definition for non-empty tuples
+    isSubterm t₁ t₂ →
+    isSubtermTuple ts₁ ts₂ →
+    isSubtermTuple (t₁ :: ts₁) (t₂ :: ts₂)
+
+-- -------------------------------------
+-- FREE VARIABLES PARA TERMOS EM L^ω_*
+-- -------------------------------------
+
+-- DEFINITION: all the (free) variables of terms in StarLang
+def freevars : Term → Finset String                           -- TODO: mudar este nome para term_vars?
+| lcons t => t.Lfreevars                                      --       since para terms: vars and free_vars it's the same
+| pi
+| sigma
+| sing
+| bUnion
+| iUnion => {}
+| var x => {x}
+| app t₁ t₂ => t₁.freevars ∪ t₂.freevars
+
+-- DEFINITION: (free) variables in tuples of terms
+--             (freevars returns the set of (free) variables)
+def freevarsTuple (tuple : TermTuple) : Finset String :=
+  (tuple.map freevars).foldl (fun acc fv => acc ∪ fv) ∅
+
+-- ---------------------------------------
+-- CLOSED TERMS
+-- ---------------------------------------
+
+def isClosedTerm (t : Term) : Prop := freevars t = {}
+def isClosedTupleTerm (t : TermTuple) : Prop := freevarsTuple t = {}
+
+-- ------------------------------------------------------------
+-- NOTATION FOR THE COMBINATORS AND THE STAR CONSTANTS IN L^ω_* (and the application of terms)
+-- ------------------------------------------------------------
+
+-- NOTATION: Notation for combinators and star constants
+notation "Π₁" => Term.pi
+notation "Σ₁" => Term.sigma
+notation "𝔰₁" => Term.sing
+notation "∪₁" => Term.bUnion
+notation "ind_⋃₁" => Term.iUnion
+notation t₁ "·" t₂ => Term.app t₁ t₂
+
+-- ------------------------------------------------------
+-- TYPECHECKING THE TERMS OF L^{omega}_*
+-- ------------------------------------------------------
+
+-- DEFINITION: Term_TypeChecking a term
+-- We typecheck the components of the formulas of L^ω_*.
+-- This guarantees that the formulas have admissible types.
+inductive Term_TypeChecking : Term → FType → Prop
+| tcLcons (t : LTerm) : Term_TypeChecking (lcons t) G                                                           -- L-constants have type G
+| tcPi {σ τ} : Term_TypeChecking pi (σ ⟶ (τ ⟶ σ))                                                             -- Π_{σ,τ} : σ ⟶ (τ ⟶ σ)
+| tcSigma {σ τ ρ}: Term_TypeChecking sigma ((σ ⟶ (τ ⟶ ρ)) ⟶ ((σ ⟶ τ) ⟶ (σ ⟶ ρ)))                           -- Σ_{σ,τ,ρ} : (σ ⟶ (τ ⟶ ρ)) ⟶ ((σ ⟶ τ) ⟶ (σ ⟶ ρ))
+| tcSing {σ}: Term_TypeChecking sing (σ ⟶ σ⋆)                                                                  -- 𝔰_{σ} : σ⋆
+| tcBUnion {σ}: Term_TypeChecking bUnion (σ⋆ ⟶ (σ⋆ ⟶ σ⋆))                                                      -- ∪_{σ} : σ⋆ ⟶ (σ⋆ ⟶ σ⋆)
+| tcIUnion {σ τ} : Term_TypeChecking iUnion (σ⋆ ⟶ ((σ ⟶ τ⋆) ⟶ τ⋆))                                            -- ∪_{σ} : σ⋆ ⟶ ((σ ⟶ τ⋆) ⟶ τ⋆)
+| tcVar {x σ}: Term_TypeChecking (var x) σ                                                                       -- Variables x : σ
+| tcApp {t₁ t₂ σ τ}: Term_TypeChecking t₁ (σ ⟶ τ) → Term_TypeChecking t₂ σ → Term_TypeChecking (app t₁ t₂) τ    -- If t₁ : (σ ⟶ τ) and t₂ : σ, then t₁t₂ : τ
+
+-- DEFINITION: Term_TypeChecking a tuple of terms
+-- Para que um tuple of terms seja typechecked checkamos se o primeiro termo tem o primeiro tipo da lista de tipos
+-- e depois o resto dos termos no tuple também têm os tipos correspondentes no resto da lista de tipos.
+inductive TermTuple_TypeChecking : TermTuple → List FType → Prop
+--| tcEmptyTuple : TermTuple_TypeChecking [] []
+| tcRecTuple {t : Term} {σ : FType} {ts : TermTuple} {σs : List FType} :
+    Term_TypeChecking t σ →
+    TermTuple_TypeChecking ts σs →
+    TermTuple_TypeChecking (t :: ts) (σ :: σs)
+
+open Term_TypeChecking
+
+
+-- -------------------------------------
+-- TERM SUBSTITUTION IN L^ω_*
+-- -------------------------------------
+
+-- Definition: term substitution, we replace x by replacement in some term t (lcons, var, app, rest)
+def term_substitution (x : String) (replacement : Term) : Term → Term
+| lcons t => match replacement with
+              | lcons r => lcons (LTerm.Lsubstitution x r t)                        -- Since replacement has to be an LTerm, we have to add this pattern matching
+              | _ => lcons t
+| var y => if x = y
+          then replacement
+          else (var y)
+| app t₁ t₂ => app (term_substitution x replacement t₁) (term_substitution x replacement t₂)  -- In an application, we do the substitution in each term
+| t => t                                                                              -- The combinators Π, Σ and the star constants 𝔰, ∪, ind_⋃ are constants and hence are not affected by substitution
+
+-- Definição de substituição de tuple terms: Substituimos _ por _ em _ (new)
+def term_substitutionTuple (x : String) (replacement : Term) : TermTuple → TermTuple
+| [] => []
+| (t :: ts) => (term_substitution x replacement t) :: term_substitutionTuple x replacement ts
+
+-- EXAMPLES: substituting in terms
+#eval term_substitution "x" Π₁ (var_x)                                        -- Replacing x by Π₁ in x gives Π₁
+#eval term_substitution "x" Π₁ (var_y)                                        -- Replacing x by Π₁ in y gives y
+#eval term_substitution "x" ∪₁ (((var_x)·(var_y))·(var_z))                    -- Replacing x by ∪₁ in (x·y)·z gives (∪₁·y)·z
+#eval term_substitution "x" (lcons (LTerm.Lvar "b")) (lcons (LTerm.Lvar "a")) -- Replacing x by (Lvariable b) in (Lvariable a) gives (Lvariable a) -> nothing happens
+
+-- EXAMPLE: substituting in tuple of terms
+-- We substitute "x" by an lconstant a in the tuple [x, (y·z)]
+#eval term_substitutionTuple "x" (lcons (Lconst_a)) [var_x, (Π₁·var_y)]       -- Output: [a, (Π₁·z)]
+
+
+-- ---------------------------------------------------------------------------------------
+
+-- ------------------
+-- FORMULAS (p.12-14)
+-- ------------------
+
+/-
+We define the formulas of L^ω_*:
+  a) The atomic formulas (definition 1.6 - p.11)
+  b) The base formulas (definition 1.10 - p.14)
+  c) The formulas (definition 1.7 - p.13)
+-/
+
+inductive Formula : Type
+| L_Form : LFormula → Formula
+| rel : String → List Term → Formula                              -- R(t₁, ..., tₙ) with R relational symbol of L and t₁,...,tₙ ground terms in L^{omega}_*
+| eq : Term → Term → Formula                                      -- t =σ q
+| mem : Term → Term → Formula                                     -- t ∈σ q
+| not : Formula → Formula                                         -- If A is a formula, then so is (¬A)
+| or : Formula → Formula → Formula                                -- If A and B are formulas, then so is (A∨B)
+| unbForall : String → Formula → Formula                        -- If A is a base formula, then so is (∀x A)
+| bForall : String → Term → Formula → Formula                     -- If A is a formula, then so is (∀x∈t A)
+deriving Repr
+--| bForall {x: String} {t:Term} {h: x ∉ t.freevars} : String → Term → Formula → Formula          -- TO DO: passar para well-formed temos de acrescentar isto
+
+-- Convertemos a lista de variáveis numa nested sequence de quantificadores `forall`
+def unbForallTuple (vars : List String) (A : Formula) : Formula :=
+  vars.foldr (fun v acc =>
+    Formula.unbForall v acc
+  ) A
+
+-- TODO: check this: do we need TermTuple?
+def bForallTuple (vars : List String) (t : Term) (A : Formula) : Formula :=
+  vars.foldr (fun v acc =>
+    Formula.bForall v t acc
+  ) A
+
+open Formula
+
+-- Helper function: well-formed FOL formulas in L^ω_*
+inductive LFormula_is_wellformed_inStar : List String → LFormula → Prop
+| wf_atomic {xs P ts} :
+    (∀ t ∈ ts, LTerm_is_wellformed_inStar xs t) →
+    LFormula_is_wellformed_inStar xs (LFormula.atomic_L P ts)                -- If t₁,...,tₙ are well-formed terms, then so is P(t₁,...,tₙ)
+| wf_not {xs A} :
+    LFormula_is_wellformed_inStar xs A →
+    LFormula_is_wellformed_inStar xs (LFormula.not_L A)                      -- If A is a well-formed formula, then so is ¬A.
+| wf_or {xs A B} :
+    LFormula_is_wellformed_inStar xs A →
+    LFormula_is_wellformed_inStar xs B →
+    LFormula_is_wellformed_inStar xs (LFormula.or_L A B)                     -- If A and B are well-formed formulas, then so is A∨B.
+| wf_forall {xs x A} :
+    LFormula_is_wellformed_inStar (x :: xs) A →
+    LFormula_is_wellformed_inStar xs (LFormula.forall_L x A)                 -- If A is a well-formed formula (for our list xs and the bound variable x), then so is ∀x A.
+
+-- Definition: well-formed formulas in L^ω_*
+inductive Formula_is_wellformed : List String → Formula → Prop
+| wf_L_Form {xs} {A : LFormula} : LFormula_is_wellformed_inStar xs A → Formula_is_wellformed xs (L_Form A)
+| wf_rel {xs P ts} :
+    (∀ t ∈ ts, Term_is_wellformed xs t) → Formula_is_wellformed xs (rel P ts)                                       -- If t₁,...,tₙ are well-formed terms, then so is P(t₁,...,tₙ)
+| wf_eq {xs t₁ t₂} :
+    Term_is_wellformed xs t₁ → Term_is_wellformed xs t₂ → Formula_is_wellformed xs (eq t₁ t₂)
+| wf_mem {xs t₁ t₂} :
+    Term_is_wellformed xs t₁ → Term_is_wellformed xs t₂ → Formula_is_wellformed xs (mem t₁ t₂)
+| wf_not {xs A} :
+    Formula_is_wellformed xs A → Formula_is_wellformed xs (not A)                                                   -- If A is a well-formed formula, then so is ¬A.
+| wf_or {xs A B} :
+    Formula_is_wellformed xs A → Formula_is_wellformed xs B → Formula_is_wellformed xs (or A B)                     -- If A and B are well-formed formulas, then so is A∨B.
+| wf_unbForall {xs x A} :
+    Formula_is_wellformed (x :: xs) A → Formula_is_wellformed xs (unbForall x A)                                    -- If A is a well-formed formula (for our list xs and the bound variable x), then so is ∀x A.
+| wf_bForall {xs x t A} :
+    Formula_is_wellformed (x :: xs) A → Formula_is_wellformed xs (bForall x t A)
+
+-- -------------------------------------
+-- FREE VARIABLES PARA FORMULAS EM L^ω_*
+-- -------------------------------------
+
+-- DEFINITION: the free variables of a formula in StarLang
+def Formula.freevars : Formula → Finset String
+| .L_Form (A : LFormula) => LFormula.Lfreevars_formula A
+| .rel _ ts => Finset.fold (fun x y => x ∪ y) {} Term.freevars ts.toFinset
+| .eq t₁ t₂
+| .mem t₁ t₂ => t₁.freevars ∪ t₂.freevars
+| .or A B => A.freevars ∪ B.freevars
+| .not A => A.freevars
+| .unbForall x A
+| .bForall x t A => A.freevars \ ([x].toFinset)
+
+
+-- DEFINITION: all the variables of a formula in StarLang
+def Formula.allvars : Formula → Finset String
+| .L_Form A => LFormula.Lallvars_formula A                                    -- The variables of a Formula are the ones of the formula when seen as an LFormula
+| .rel _ ts => Finset.fold (fun x y => x ∪ y) {} Term.freevars ts.toFinset    -- All the variables from the list of terms used in the predicate
+| .eq t₁ t₂
+| .mem t₁ t₂ => t₁.freevars ∪ t₂.freevars                                     -- For both terms, we collect the variables from both and consider the union of those sets
+| .or A B => A.allvars ∪ B.allvars                                            -- Take the variables from both subformulas and consider the union of those sets
+| .not A => A.allvars                                                         -- The variables of ¬A are the ones of A
+| .unbForall x A => A.allvars ∪ {x}                                           -- The variables of ∀x A are the ones of A together with the bound variable
+| .bForall x t A => t.freevars ∪ A.allvars ∪ {x}                              -- The variables of ∀x∈t A are the ones of A together with the bound variable and the variables in t
+
+-- Example after notation
+
+/-
+With these definitions, we can create assumptions such as:
+    x is a free variable of formula A       -> In Lean: x ∈ A.freevars
+    x is not a free variable of formula A   -> In Lean: x ∉ A.freevars
+
+    x is a variable of formula A            -> In Lean: x ∈ A.allvars
+    x is not a variable of formula A        -> In Lean: x ∉ A.allvars
+-/
+
+-- -------------------------
+-- NOTATION: PRIMITE SYMBOLS
+-- -------------------------
+
+-- NOTATION: Notation for the equality and the membership symbols
+notation t₁ "=₁" t₂ => Formula.eq t₁ t₂
+notation t₁ "∈₁" t₂ => Formula.mem t₁ t₂
+
+-- NOTATION: Notation for the primitive symbols ¬, ∨, ∀x and ∀x∈t in L^{omega}_*
+notation "¬₁" A => not A
+notation A "∨₁" B => or A B
+notation "∀₁₁" => unbForall
+notation "b∀₁₁" => bForall
+notation "∀₁" => unbForallTuple
+notation "b∀₁" => bForallTuple
+
+-- DEFINITION 1.8 (p.14): The bounded existential quantifier ∃x∈t (defined symbol)
+
+-- The unbounded existential quantifier (for one variable): ∃x A := ¬ (∀x (¬ A))
+@[simp]
+def unbExists (x : String) (A : Formula) : Formula :=
+  ¬₁(unbForall x (¬₁ A))
+
+-- The bounded existential quantifier (for one variable) ∃x∈t A := ¬ (∀x∈t (¬ A))
+@[simp]
+def bExists (x : String) (t : Term) (A : Formula) : Formula :=
+  ¬₁(bForall x t (¬₁ A))
+
+-- The unbounded existential quantifier (for a tuple of variables):  ∃x A := ¬ (∀x (¬ A))
+@[simp]
+def unbExistsTuple (x : List String) (A : Formula) : Formula :=
+  ¬₁ (∀₁ x (¬₁A))
+
+-- The bounded existential quantifier (for a tuple of variables):  ∃x∈t A := ¬ (∀x∈t (¬ A))
+@[simp]
+def bExistsTuple (x : List String) (t : Term) (A : Formula) : Formula :=
+  ¬₁ (b∀₁ x t (¬₁A))
+
+notation "∃₁₁" => unbExists
+notation "b∃₁₁" => bExists
+notation "∃₁" => unbExistsTuple
+notation "b∃₁" => bExistsTuple
+
+-- -------------------------
+-- NOTATION: DEFINED SYMBOLS (p.8 and p.14):
+-- Usual logical abbreviations for the defined symbols ∧, →, ↔, ∃x and ∃x∈t in L^{omega}_*
+-- -------------------------
+
+-- Conjunction:  A ∧ B := ¬(¬A∨¬B)
+@[simp]
+def F_and (A B : Formula) : Formula :=
+  ¬₁ ((¬₁ A) ∨₁ (¬₁ B))
+
+notation A "∧₁" B => F_and A B
+
+-- Implication:  A → B := ¬ A ∨ B
+@[simp]
+def F_implies (A B : Formula) : Formula :=
+  (¬₁ A) ∨₁ B
+
+notation A "→₁" B => F_implies A B
+
+-- Equivalence:  A ↔ B := (A → B) ∧ (B → A)
+@[simp]
+def F_iff (A B : Formula) : Formula :=
+  ¬₁ ((¬₁((¬₁A) ∨₁ B)) ∨₁ (¬₁((¬₁B) ∨₁ A)))
+  -- (A →₁ B) ∧₁ (B →₁ A)
+  -- (¬₁ A ∨₁ B) ∧₁ (¬₁ B ∨₁ A)
+
+notation A "↔₁" B => F_iff A B
+
+-- EXAMPLE OF FREE VARIABLES AND VARIABLES OF A FORMULA
+-- Formula R(x,y) ∨ (∀z∈t Q(z)) - Free variables and check whether sentence
+def ex_freevars_formula := (rel "R" [var "x", var "y"]) ∨₁ (b∀₁₁ "z" (var "t") (rel "Q" [var "z"]))
+#eval Formula.freevars ex_freevars_formula            -- The set of free variables is the set {x,y}, that is {"x", "y"}
+#eval Formula.allvars ex_freevars_formula             -- TODO: aqui aparece t como variável, é preciso mudar var "t" aqui e nos exemplos em baixo
+
+
+-- ----------------------------
+-- SENTENCES (CLOSED FORMULAS)
+-- ----------------------------
+
+def isClosed (A : Formula) : Prop := Formula.freevars A = {}
+def isClosed_check (A : Formula) : Bool := (Formula.freevars A) = {}       -- Prints true or false dependendo se temos var livres ou não
+
+-- EXAMPLE 1: Formula R(x,y) ∨ (∀z∈t Q(z)) - Free variables and check whether sentence
+def ex1_freevars_formula := (rel "R" [var "x", var "y"]) ∨₁ (b∀₁₁ "z" (var "t") (rel "Q" [var "z"]))
+#eval Formula.freevars ex1_freevars_formula                         -- The set of free variables is the set {x,y}, that is {"x", "y"}
+#eval isClosed_check ex1_freevars_formula                           -- Since ex1_freevars_formula has x and y as free variables, the output is false
+
+-- EXAMPLE 2: Formula R(x,y) - Free variables and check whether sentence
+def ex2_freevars_formula := (rel "R" [var "x", var "y"])
+#eval Formula.freevars ex2_freevars_formula                         -- The set of free variables is the set {x,y}, that is {"x", "y"}
+#eval isClosed_check ex2_freevars_formula                           -- Since ex2_freevars_formula has x and y as free variables, the output is false
+
+-- EXAMPLE 3: Formula ∀z∈t Q(z) - Free variables and check whether sentence
+def ex3_freevars_formula := (b∀₁₁ "z" (var "t") (rel "Q" [var "z"]))
+#eval Formula.freevars ex3_freevars_formula                         -- The set of free variables is the empty set ∅
+#eval isClosed_check ex3_freevars_formula                           -- Since ex3_freevars_formula has no free variables, the output is true
+
+
+-- ------------------------------------------------------
+-- CHECKING FORMULAS:
+-- ------------------------------------------------------
+
+-- Checks whether a given formula is atomic:
+inductive isAtomic : Formula → Prop
+| at_rel : isAtomic (rel x l_term)
+| at_eq : isAtomic (eq t₁ t₂)
+| at_mem : isAtomic (mem t₁ t₂)
+
+-- Checks whether a given formula is base:
+inductive isBase : Formula → Prop
+| b_atom : isAtomic A → isBase A                                                -- Atomic formulas are base formulas
+| b_not (h: isBase A) : isBase (not A)                                          -- If A is base, then so is ¬₁A
+| b_or (h1: isBase A) (h2 : isBase B) : isBase (or A B)                         -- If A and B are base, then so is A∨₁B
+| b_bForall (x : String) (t : Term) (h : isBase A) : isBase (bForall x t A)     -- If A is base, then so is ∀x∈t A
+
+open isBase
+
+-- Example: Let A be an atomic formula (assumption h), then it is base.
+example (A : Formula) (h : isAtomic A)  : (isBase A) := by
+  exact b_atom h
+
+example (A B : Formula) (hA_at : isAtomic A) (hB_b : isBase B) : (isBase (A∨₁B)) := by
+  have h := b_atom hA_at
+  exact b_or h hB_b
+
+
+
+
+-- --------------------------------------------------------------------------
+-- LEMMAS: Defined symbols of base formulas are also base (Remark 1.11, p.14)
+-- --------------------------------------------------------------------------
+
+-- Lemma Conj_base states that if A and B are base formulas, then so is their conjunction A ∧ B
+lemma Conj_base (A B : Formula) (hA : isBase A) (hB : isBase B) : (isBase (A∧₁B)) := by
+  unfold F_and
+  have h_nA := b_not hA
+  have h_nB := b_not hB
+  have h_or_nAnB := b_or h_nA h_nB
+  exact b_not h_or_nAnB
+
+-- Lemma Imp_base states that if A and B are base formulas, then so is their implication A → B
+lemma Imp_base (A B : Formula) (hA : isBase A) (hB : isBase B) : (isBase (A→₁B)) := by
+  unfold F_implies
+  have h_nA := b_not hA
+  exact b_or h_nA hB
+
+-- Lemma Iff_base states that if A and B are base formulas, then so is their equivalence A ↔ B
+lemma Iff_base (A B : Formula) (hA : isBase A) (hB : isBase B) : (isBase (A↔₁B)) := by
+  unfold F_iff
+  have h_nA := b_not hA
+  have h_nB := b_not hB
+  have h_or_nAB := b_or h_nA hB
+  have h_or_nBA := b_or h_nB hA
+  have h_n_or_nAB := b_not h_or_nAB
+  have h_n_or_nBA := b_not h_or_nBA
+  have H := b_or h_n_or_nAB h_n_or_nBA
+  exact b_not H
+
+-- Lemma unbForall_base states that if A is a base formula, then so is ∃x∈t A
+lemma bExists_base {A : Formula} (x : String) (t : Term) (hA : isBase A) : (isBase (b∃₁₁ x t A)) := by
+  unfold bExists
+  have h_nA := b_not hA
+  have h_unbForall_nA := b_bForall x t h_nA
+  exact b_not h_unbForall_nA
+
+-- ------------------
+-- EXAMPLE 1.6 (p.14)
+-- ------------------
+
+-- Example 1.6.1 (p.14): If B is a base formula, then so is ∀x∈t B(x)
+example (B : Formula) (hB_b : isBase B) (x : String) (t : Term): (isBase (b∀₁₁ x t (¬₁ B))) := by
+  have H := b_not hB_b
+  exact b_bForall x t H
+
+-- Example 1.6.2 (p.14): If A and B are base formulas, then so is ∀x∈t ∃y∈q (A∨B)
+example (A B : Formula) (hA_b : isBase A) (hB_b : isBase B) (x y : String) (t q : Term): (isBase (b∀₁₁ x t (b∃₁₁ y q (A ∨₁ B)))) := by
+  have H_or_AB := b_or hA_b hB_b
+  have H_bExists := bExists_base y q H_or_AB
+  exact b_bForall x t H_bExists
+
+-- ------------------------------------------------------
+-- TYPECHECKING
+-- We typecheck the components of the formulas of L^ω_*.
+-- This guarantees that the formulas have admissible types.
+-- ------------------------------------------------------
+
+inductive Formula_TypeChecking : Formula → Prop
+| tcRel {R l_terms} :                                               -- R é relational symbol DE L (falta); l_terms é uma lista de termos
+    (∀ t, t ∈ l_terms → Term_TypeChecking t G) →
+    Formula_TypeChecking (Formula.rel R l_terms)
+| tcEq {σ t₁ t₂} :
+    Term_TypeChecking t₁ σ →
+    Term_TypeChecking t₂ σ →
+    Formula_TypeChecking (Formula.eq t₁ t₂)
+| tcMem {σ t₁ t₂} :
+    Term_TypeChecking t₁ σ →
+    Term_TypeChecking t₂ (σ⋆) →
+    Formula_TypeChecking (Formula.mem t₁ t₂)
+| tcNot {A} :
+    Formula_TypeChecking A → Formula_TypeChecking (Formula.not A)
+| tcOr {A B} :
+    Formula_TypeChecking A →
+    Formula_TypeChecking B →
+    Formula_TypeChecking (Formula.or A B)
+| tcbForall {x σ t A} :
+    Term_TypeChecking (Term.var x) σ →
+    Term_TypeChecking t (σ⋆) →
+    Formula_TypeChecking A →
+    Formula_TypeChecking (Formula.bForall x t A)
+| tcunbForall {x σ A} :
+    Term_TypeChecking (Term.var x) σ →
+    Formula_TypeChecking A →
+    Formula_TypeChecking (Formula.unbForall x A)
+
+-- -------------------------------------
+-- FORMULA SUBSTITUTION IN L^ω_*
+-- -------------------------------------
+
+def substitution_formula (x : String) (replacement : Term) : Formula → Formula
+| (L_Form A) => match replacement with
+              | .lcons r => L_Form (LFormula.Lsubstitution_formula x r A)
+              | _ => (L_Form A)
+| (rel P terms) => rel P (terms.map (term_substitution x replacement))
+| (t₁ =₁ t₂) => (term_substitution x replacement t₁) =₁ (term_substitution x replacement t₂)
+| (t₁ ∈₁ t₂) => (term_substitution x replacement t₁) ∈₁ (term_substitution x replacement t₂)
+| (Formula.not A) => ¬₁ (substitution_formula x replacement A)                                                       -- recursivamente em A
+| (Formula.or A B) => (substitution_formula x replacement A) ∨₁ (substitution_formula x replacement B)               -- recursivamente em A e B
+| (∀₁₁ y A) => if x = y then ∀₁₁ y A
+              else ∀₁₁ y (substitution_formula x replacement A)
+| (b∀₁₁ y t A) => if x = y then b∀₁₁ y t A
+              else (b∀₁₁ y t (substitution_formula x replacement A))
+
+
+-- EXAMPLES: formula substitution           -- TODO: falta o repr para podermos ter estes examplos com #eval
+
+-- Example 1:
+#eval substitution_formula "x" Π₁ (rel "R" [var_x, var_y])        -- Output: R(Π₁,y)
+
+-- Example 2:
+def ex2_subst : Formula :=
+    (¬₁( (var "x")∈₁(var "y") )) ∨₁ ((var "z")=₁(var "w"))
+#eval substitution_formula "z" ∪₁ ex2_subst                       -- Output: (¬₁(x ∈₁ y)) ∨₁ (∪₁ =₁ w)
+
+-- Example 3:
+def ex3_subst : Formula :=
+  bForall "y" (var "a") ((var "x")=₁(var "y"))
+#eval substitution_formula "x" ind_⋃₁ ex3_subst                   -- Output: ∀ y ∈ a (ind_⋃₁ =₁ y)
+
+
+/- Próximas tarefas:
+      1. Truly check a cena do ∀x∈t, what is tuple, what is not and how to interpretar
+      2. Fazer fórmulas com A(t) em que t é fórmula and how to interpretar
+          + o que tem de ser alterado nas defs das fórmulas
+      3. Fazer simultaneous substitution (terms and formulas)
+      4. Prenexificação aqui
+-/
